VsaIris.lean
@@ -71,6 +71,7 @@ import VsaIris.Interp.SpecEval
 import VsaIris.Interp.Arm
 import VsaIris.Interp.SeqLoop
 import VsaIris.Interp.SeqLoopClosure
+import VsaIris.Interp.SeqLoopInterp
 import VsaIris.Interp.Case.BinaryAddIntT
 import VsaIris.Interp.Case.BinarySubIntT
 import VsaIris.Interp.Case.BinaryAddIntP
